proof/invariant-abstract/ARM/Machine_AI.thy
@@ -336,7 +336,9 @@ lemma no_fail_ackInterrupt[wp]: "no_fail \<top> (ackInterrupt irq)"
 lemma no_fail_maskInterrupt[wp]: "no_fail \<top> (maskInterrupt irq bool)"
   by (simp add: maskInterrupt_def)
 
-
+lemma no_fail_sendSGI[wp]:
+  "no_fail \<top> (sendSGI irq target)"
+  by (simp add: sendSGI_def)
 
 lemma no_irq_use:
   "\<lbrakk> no_irq f; (rv,s') \<in> fst (f s) \<rbrakk> \<Longrightarrow> irq_masks s' = irq_masks s"
@@ -358,6 +360,10 @@ crunch machine_op_lift
 lemma no_irq:
   "no_irq f \<Longrightarrow> \<lbrace>\<lambda>s. P (irq_masks s)\<rbrace> f \<lbrace>\<lambda>_ s. P (irq_masks s)\<rbrace>"
   by (simp add: no_irq_def)
+
+lemma no_irq_sendSGI:
+  "no_irq (sendSGI irq target)"
+  by (simp add: sendSGI_def)
 
 lemma no_irq_isb: "no_irq  isb"
   by (simp add: isb_def)
@@ -642,6 +648,10 @@ lemma empty_fail_dsb: "empty_fail  dsb"
 
 lemma empty_fail_dmb: "empty_fail  dmb"
   by (simp add: dmb_def)
+
+lemma empty_fail_sendSGI:
+  "empty_fail (sendSGI irq target)"
+  by (simp add: sendSGI_def)
 
 lemma empty_fail_cleanByVA: "empty_fail  (cleanByVA w p)"
   by (simp add: cleanByVA_def)
